SP1Chips.lean
@@ -1,4 +1,5 @@
 import SP1Chips.AddChip
 import SP1Chips.BitwiseChip
 import SP1Chips.JalChip
+import SP1Chips.MulChip
 import SP1Chips.SubChip
