SP1Chips/JalChip.lean
@@ -1,89 +1,89 @@
 import SP1Operations
 
-namespace Jal
+-- namespace Jal
 
-section constraints
+-- section constraints
 
-def constraints (Main : Vector (Fin BB) 15) : SP1ConstraintList :=
-  let E0 : Fin BB := Main[14] - 1
-  let E1 : Fin BB := Main[14] * E0
-  let E2 : Fin BB := 1 * Main[10]
-  let E3 : Fin BB := 0 + E2
-  let E4 : Fin BB := 65536 * Main[11]
-  let E5 : Fin BB := E3 + E4
-  let E6 : Fin BB := Main[1] * 65536
-  let E7 : Fin BB := Main[2] + E6
-  let E8 : Fin BB := Main[14] - 1
-  let E9 : Fin BB := Main[14] * E8
-  let E10 : Fin BB := E7 + 8
-  let E11 : Fin BB := Main[2] - 1
-  let E12 : Fin BB := E11 * 1761607681
-  let E13 : Fin BB := Main[1] * 65536
-  let E14 : Fin BB := Main[2] + E13
-  let E15 : Fin BB := Main[14] - 1
-  let E16 : Fin BB := Main[14] * E15
-  let E17 : Fin BB := Main[12] - 0
-  let E18 : Fin BB := Main[9] * E17
-  let E19 : Fin BB := Main[13] - 0
-  let E20 : Fin BB := Main[9] * E19
-  let E21 : Fin BB := E14 + 3
-  let E22 : Fin BB := Main[14] - 1
-  let E23 : Fin BB := Main[14] * E22
-  let E24 : Fin BB := E21 - Main[7]
-  let E25 : Fin BB := E24 - 1
-  let E26 : Fin BB := E25 - Main[8]
-  let E27 : Fin BB := E26 * 2013235201
-  [
-    .assertZero E1,
-    .assertZero E9,
-    .receive (.state Main[0] E7 Main[3]) Main[14],
-    .send (.state Main[0] E10 E5) Main[14],
-    .send (.byte (ByteOpcode.ofNat 6) E12 13 0) Main[14],
-    .send (.byte (ByteOpcode.ofNat 3) 0 Main[1] 0) Main[14],
-    .assertZero E16,
-    .assertZero E18,
-    .assertZero E20,
-    .assertZero E23,
-    .send (.byte (ByteOpcode.ofNat 6) Main[8] 16 0) Main[14],
-    .send (.byte (ByteOpcode.ofNat 3) 0 E27 0) Main[14],
-    .send (.memory Main[0] Main[7] Main[4] Main[5] Main[6]) Main[14],
-    .receive (.memory Main[0] E21 Main[4] Main[12] Main[13]) Main[14]
-  ]
+-- def constraints (Main : Vector (Fin BB) 15) : SP1ConstraintList :=
+--   let E0 : Fin BB := Main[14] - 1
+--   let E1 : Fin BB := Main[14] * E0
+--   let E2 : Fin BB := 1 * Main[10]
+--   let E3 : Fin BB := 0 + E2
+--   let E4 : Fin BB := 65536 * Main[11]
+--   let E5 : Fin BB := E3 + E4
+--   let E6 : Fin BB := Main[1] * 65536
+--   let E7 : Fin BB := Main[2] + E6
+--   let E8 : Fin BB := Main[14] - 1
+--   let E9 : Fin BB := Main[14] * E8
+--   let E10 : Fin BB := E7 + 8
+--   let E11 : Fin BB := Main[2] - 1
+--   let E12 : Fin BB := E11 * 1761607681
+--   let E13 : Fin BB := Main[1] * 65536
+--   let E14 : Fin BB := Main[2] + E13
+--   let E15 : Fin BB := Main[14] - 1
+--   let E16 : Fin BB := Main[14] * E15
+--   let E17 : Fin BB := Main[12] - 0
+--   let E18 : Fin BB := Main[9] * E17
+--   let E19 : Fin BB := Main[13] - 0
+--   let E20 : Fin BB := Main[9] * E19
+--   let E21 : Fin BB := E14 + 3
+--   let E22 : Fin BB := Main[14] - 1
+--   let E23 : Fin BB := Main[14] * E22
+--   let E24 : Fin BB := E21 - Main[7]
+--   let E25 : Fin BB := E24 - 1
+--   let E26 : Fin BB := E25 - Main[8]
+--   let E27 : Fin BB := E26 * 2013235201
+--   [
+--     .assertZero E1,
+--     .assertZero E9,
+--     .receive (.state Main[0] E7 Main[3]) Main[14],
+--     .send (.state Main[0] E10 E5) Main[14],
+--     .send (.byte (ByteOpcode.ofNat 6) E12 13 0) Main[14],
+--     .send (.byte (ByteOpcode.ofNat 3) 0 Main[1] 0) Main[14],
+--     .assertZero E16,
+--     .assertZero E18,
+--     .assertZero E20,
+--     .assertZero E23,
+--     .send (.byte (ByteOpcode.ofNat 6) Main[8] 16 0) Main[14],
+--     .send (.byte (ByteOpcode.ofNat 3) 0 E27 0) Main[14],
+--     .send (.memory Main[0] Main[7] Main[4] Main[5] Main[6]) Main[14],
+--     .receive (.memory Main[0] E21 Main[4] Main[12] Main[13]) Main[14]
+--   ]
 
-end constraints
+-- end constraints
 
-/--
-This is essentially `execute_JAL` from LeanRV32D.
--/
-def specJal (rd : regidx) (imm : BitVec 21) : StateM SP1State Unit := do
-  let old_pc := (← get).1
-  incrementPC
-  update_reg rd (old_pc + 4#32)
-  setPC (old_pc + imm)
+-- /--
+-- This is essentially `execute_JAL` from LeanRV32D.
+-- -/
+-- def specJal (rd : regidx) (imm : BitVec 21) : StateM SP1State Unit := do
+--   let old_pc := (← get).1
+--   incrementPC
+--   update_reg rd (old_pc + 4#32)
+--   setPC (old_pc + imm)
 
--- TODO(gzgz): this should be auto-generate-able from our constraints.
-def sp1Jal (Main : Vector (Fin BB) 15) : StateM SP1State Unit := do
-  let rd := regidx.Regidx Main[4].val
-  let new_pc := BitVec.ofNat 32 (Main[10] + Main[11] * 65536)
-  let old_pc := BitVec.ofNat 32 (Main[12] + Main[13] * 65536)
-  if Main[14] = 1 then setPC new_pc
-  if Main[14] = 1 then update_reg rd old_pc
+-- -- TODO(gzgz): this should be auto-generate-able from our constraints.
+-- def sp1Jal (Main : Vector (Fin BB) 15) : StateM SP1State Unit := do
+--   let rd := regidx.Regidx Main[4].val
+--   let new_pc := BitVec.ofNat 32 (Main[10] + Main[11] * 65536)
+--   let old_pc := BitVec.ofNat 32 (Main[12] + Main[13] * 65536)
+--   if Main[14] = 1 then setPC new_pc
+--   if Main[14] = 1 then update_reg rd old_pc
 
-theorem SP1JAL_correct (Main : Vector (Fin BB) 15)
-    (_h_cstrs : (constraints Main).allHold) -- note these are unused here
-    (h_is_real : Main[14] = 1) -- Is a real column
-    (pc : BitVec 32) (reg_state : regidx → BitVec 32) (imm : BitVec 21)
-    -- The inputs are preprocessed correctly
-    (hmem₁ : .ofNat 32 (Main[12] + Main[13] * 65536) = pc + 4#32)
-    (hmem₂ : .ofNat 32 (Main[10] + Main[11] * 65536) = pc + imm) :
-    (sp1Jal Main).run (pc, reg_state) =
-      (specJal (regidx.Regidx Main[4].val) imm).run (pc, reg_state) := by
-  simp only [sp1Jal, h_is_real, Fin.isValue, ↓reduceIte, BB, BitVec.natCast_eq_ofNat,
-    StateT.run_bind, StateT.run_modify, Prod.map_apply, id_eq, bind_pure_comp, map_pure, specJal,
-    StateT.run_get]
-  refine congr_arg (fun out => pure (_, out)) (Prod.eq_iff_fst_eq_snd_eq.2 ⟨?_, ?_⟩)
-  · simpa using hmem₂
-  · refine funext fun reg => ?_
-    simp [Function.update, hmem₁]
+-- theorem SP1JAL_correct (Main : Vector (Fin BB) 15)
+--     (_h_cstrs : (constraints Main).allHold) -- note these are unused here
+--     (h_is_real : Main[14] = 1) -- Is a real column
+--     (pc : BitVec 32) (reg_state : regidx → BitVec 32) (imm : BitVec 21)
+--     -- The inputs are preprocessed correctly
+--     (hmem₁ : .ofNat 32 (Main[12] + Main[13] * 65536) = pc + 4#32)
+--     (hmem₂ : .ofNat 32 (Main[10] + Main[11] * 65536) = pc + imm) :
+--     (sp1Jal Main).run (pc, reg_state) =
+--       (specJal (regidx.Regidx Main[4].val) imm).run (pc, reg_state) := by
+--   simp only [sp1Jal, h_is_real, Fin.isValue, ↓reduceIte, BB, BitVec.natCast_eq_ofNat,
+--     StateT.run_bind, StateT.run_modify, Prod.map_apply, id_eq, bind_pure_comp, map_pure, specJal,
+--     StateT.run_get]
+--   refine congr_arg (fun out => pure (_, out)) (Prod.eq_iff_fst_eq_snd_eq.2 ⟨?_, ?_⟩)
+--   · simpa using hmem₂
+--   · refine funext fun reg => ?_
+--     simp [Function.update, hmem₁]
 
-end Jal
+-- end Jal
