SP1Foundations.lean
@@ -2,6 +2,7 @@ import SP1Foundations.BitVec
 import SP1Foundations.ByteOpcode
 import SP1Foundations.Constraint
 import SP1Foundations.Field
+import SP1Foundations.MemoryConsistency
 import SP1Foundations.Misc
 import SP1Foundations.SP1State
 import SP1Foundations.SailM
