SP1Operations/ALUTypeReader.lean
@@ -1,180 +1,180 @@
-import SP1Foundations
-import SP1Operations.MemoryConsistency
-import LeanRV32IM.RiscvRegs
+-- import SP1Foundations
+-- import SP1Operations.MemoryConsistency
+-- import LeanRV32IM.RiscvRegs
 
-open LeanRV32IM.Functions
+-- open LeanRV32IM.Functions
 
---- A Reader that only accesses values of type `T`.
-structure ALUTypeReader where
-  op_a : Fin BB
-  op_a_memory : MemoryAccessInSharedCols
-  op_a_0 : Fin BB
-  op_b : Fin BB
-  op_b_memory : MemoryAccessInSharedCols
-  op_c : Word (Fin BB)
-  op_c_memory : MemoryAccessInSharedCols
-  imm_c : Fin BB
+-- --- A Reader that only accesses values of type `T`.
+-- structure ALUTypeReader where
+--   op_a : Fin BB
+--   op_a_memory : MemoryAccessInSharedCols
+--   op_a_0 : Fin BB
+--   op_b : Fin BB
+--   op_b_memory : MemoryAccessInSharedCols
+--   op_c : Word (Fin BB)
+--   op_c_memory : MemoryAccessInSharedCols
+--   imm_c : Fin BB
 
-namespace ALUTypeReader
+-- namespace ALUTypeReader
 
-def constraints
-  (shard clk _pc _opcode: Fin BB)
-  (op_a_write_value : Word (Fin BB))
-  (cols : ALUTypeReader)
-  (is_real : Fin BB)
-  : SP1ConstraintList :=
-    let E0 : Fin BB := is_real - 1
-    let E2 : Fin BB := is_real * E0
-    let E4 : Fin BB := is_real - 1
-    let E6 : Fin BB := cols.imm_c - 0
-    let E8 : Fin BB := E4 * E6
-    let E10 : Fin BB := 0 + cols.op_b
-    let E12 : Fin BB := op_a_write_value[0] - 0
-    let E14 : Fin BB := cols.op_a_0 * E12
-    let E16 : Fin BB := op_a_write_value[1] - 0
-    let E18 : Fin BB := cols.op_a_0 * E16
-    let E20 : Fin BB := clk + 3
-    let E22 : Fin BB := is_real - 1
-    let E24 : Fin BB := is_real * E22
-    let E26 : Fin BB := E20 - cols.op_a_memory.access_timestamp.prev_low
-    let E28 : Fin BB := E26 - 1
-    let E30 : Fin BB := E28 - cols.op_a_memory.access_timestamp.diff_low_limb
-    let E32 : Fin BB := E30 * 2013143041
-    let E34 : Fin BB := clk + 2
-    let E36 : Fin BB := is_real - 1
-    let E38 : Fin BB := is_real * E36
-    let E40 : Fin BB := E34 - cols.op_b_memory.access_timestamp.prev_low
-    let E42 : Fin BB := E40 - 1
-    let E44 : Fin BB := E42 - cols.op_b_memory.access_timestamp.diff_low_limb
-    let E46 : Fin BB := E44 * 2013143041
-    let E48 : Fin BB := clk + 1
-    let E50 : Fin BB := is_real - cols.imm_c
-    let E52 : Fin BB := E50 - 1
-    let E54 : Fin BB := E50 * E52
-    let E56 : Fin BB := E48 - cols.op_c_memory.access_timestamp.prev_low
-    let E58 : Fin BB := E56 - 1
-    let E60 : Fin BB := E58 - cols.op_c_memory.access_timestamp.diff_low_limb
-    let E62 : Fin BB := E60 * 2013143041
-    let E64 : Fin BB := cols.op_c_memory.prev_value[0] - cols.op_c[0]
-    let E66 : Fin BB := cols.imm_c * E64
-    let E68 : Fin BB := cols.op_c_memory.prev_value[1] - cols.op_c[1]
-    let E70 : Fin BB := cols.imm_c * E68
+-- def constraints
+--   (shard clk _pc _opcode: Fin BB)
+--   (op_a_write_value : Word (Fin BB))
+--   (cols : ALUTypeReader)
+--   (is_real : Fin BB)
+--   : SP1ConstraintList :=
+--     let E0 : Fin BB := is_real - 1
+--     let E2 : Fin BB := is_real * E0
+--     let E4 : Fin BB := is_real - 1
+--     let E6 : Fin BB := cols.imm_c - 0
+--     let E8 : Fin BB := E4 * E6
+--     let E10 : Fin BB := 0 + cols.op_b
+--     let E12 : Fin BB := op_a_write_value[0] - 0
+--     let E14 : Fin BB := cols.op_a_0 * E12
+--     let E16 : Fin BB := op_a_write_value[1] - 0
+--     let E18 : Fin BB := cols.op_a_0 * E16
+--     let E20 : Fin BB := clk + 3
+--     let E22 : Fin BB := is_real - 1
+--     let E24 : Fin BB := is_real * E22
+--     let E26 : Fin BB := E20 - cols.op_a_memory.access_timestamp.prev_low
+--     let E28 : Fin BB := E26 - 1
+--     let E30 : Fin BB := E28 - cols.op_a_memory.access_timestamp.diff_low_limb
+--     let E32 : Fin BB := E30 * 2013143041
+--     let E34 : Fin BB := clk + 2
+--     let E36 : Fin BB := is_real - 1
+--     let E38 : Fin BB := is_real * E36
+--     let E40 : Fin BB := E34 - cols.op_b_memory.access_timestamp.prev_low
+--     let E42 : Fin BB := E40 - 1
+--     let E44 : Fin BB := E42 - cols.op_b_memory.access_timestamp.diff_low_limb
+--     let E46 : Fin BB := E44 * 2013143041
+--     let E48 : Fin BB := clk + 1
+--     let E50 : Fin BB := is_real - cols.imm_c
+--     let E52 : Fin BB := E50 - 1
+--     let E54 : Fin BB := E50 * E52
+--     let E56 : Fin BB := E48 - cols.op_c_memory.access_timestamp.prev_low
+--     let E58 : Fin BB := E56 - 1
+--     let E60 : Fin BB := E58 - cols.op_c_memory.access_timestamp.diff_low_limb
+--     let E62 : Fin BB := E60 * 2013143041
+--     let E64 : Fin BB := cols.op_c_memory.prev_value[0] - cols.op_c[0]
+--     let E66 : Fin BB := cols.imm_c * E64
+--     let E68 : Fin BB := cols.op_c_memory.prev_value[1] - cols.op_c[1]
+--     let E70 : Fin BB := cols.imm_c * E68
 
-    [
-      .assertZero E2,
-      .assertZero E8,
-      .assertZero E14,
-      .assertZero E18,
-      .assertZero E24,
-      .send (.byte (ByteOpcode.ofNat 6) cols.op_a_memory.access_timestamp.diff_low_limb 14 0) is_real,
-      .send (.byte (ByteOpcode.ofNat 6) E32 14 0) is_real,
-      .send (.memory shard cols.op_a_memory.access_timestamp.prev_low cols.op_a cols.op_a_memory.prev_value[0] cols.op_a_memory.prev_value[1]) is_real,
-      .receive (.memory shard E20 cols.op_a op_a_write_value[0] op_a_write_value[1]) is_real,
-      .assertZero E38,
-      .send (.byte (ByteOpcode.ofNat 6) cols.op_b_memory.access_timestamp.diff_low_limb 14 0) is_real,
-      .send (.byte (ByteOpcode.ofNat 6) E46 14 0) is_real,
-      .send (.memory shard cols.op_b_memory.access_timestamp.prev_low cols.op_b cols.op_b_memory.prev_value[0] cols.op_b_memory.prev_value[1]) is_real,
-      .receive (.memory shard E34 cols.op_b cols.op_b_memory.prev_value[0] cols.op_b_memory.prev_value[1]) is_real,
-      .assertZero E54,
-      .send (.byte (ByteOpcode.ofNat 6) cols.op_c_memory.access_timestamp.diff_low_limb 14 0) E50,
-      .send (.byte (ByteOpcode.ofNat 6) E62 14 0) E50,
-      .send (.memory shard cols.op_c_memory.access_timestamp.prev_low cols.op_c[0] cols.op_c_memory.prev_value[0] cols.op_c_memory.prev_value[1]) E50,
-      .receive (.memory shard E48 cols.op_c[0] cols.op_c_memory.prev_value[0] cols.op_c_memory.prev_value[1]) E50,
-      .assertZero E66,
-      .assertZero E70
-    ]
+--     [
+--       .assertZero E2,
+--       .assertZero E8,
+--       .assertZero E14,
+--       .assertZero E18,
+--       .assertZero E24,
+--       .send (.byte (ByteOpcode.ofNat 6) cols.op_a_memory.access_timestamp.diff_low_limb 14 0) is_real,
+--       .send (.byte (ByteOpcode.ofNat 6) E32 14 0) is_real,
+--       .send (.memory shard cols.op_a_memory.access_timestamp.prev_low cols.op_a cols.op_a_memory.prev_value[0] cols.op_a_memory.prev_value[1]) is_real,
+--       .receive (.memory shard E20 cols.op_a op_a_write_value[0] op_a_write_value[1]) is_real,
+--       .assertZero E38,
+--       .send (.byte (ByteOpcode.ofNat 6) cols.op_b_memory.access_timestamp.diff_low_limb 14 0) is_real,
+--       .send (.byte (ByteOpcode.ofNat 6) E46 14 0) is_real,
+--       .send (.memory shard cols.op_b_memory.access_timestamp.prev_low cols.op_b cols.op_b_memory.prev_value[0] cols.op_b_memory.prev_value[1]) is_real,
+--       .receive (.memory shard E34 cols.op_b cols.op_b_memory.prev_value[0] cols.op_b_memory.prev_value[1]) is_real,
+--       .assertZero E54,
+--       .send (.byte (ByteOpcode.ofNat 6) cols.op_c_memory.access_timestamp.diff_low_limb 14 0) E50,
+--       .send (.byte (ByteOpcode.ofNat 6) E62 14 0) E50,
+--       .send (.memory shard cols.op_c_memory.access_timestamp.prev_low cols.op_c[0] cols.op_c_memory.prev_value[0] cols.op_c_memory.prev_value[1]) E50,
+--       .receive (.memory shard E48 cols.op_c[0] cols.op_c_memory.prev_value[0] cols.op_c_memory.prev_value[1]) E50,
+--       .assertZero E66,
+--       .assertZero E70
+--     ]
 
-/-- `.assertZero E2` (also `E22`) -/
-lemma is_real_eq_of_constraints
-    (h : (constraints shard clk pc opcode op_a_write_value cols is_real).allHold) :
-    is_real = 0 ∨ is_real = 1 := by
-  simp_all [constraints, sub_eq_zero]
+-- /-- `.assertZero E2` (also `E22`) -/
+-- lemma is_real_eq_of_constraints
+--     (h : (constraints shard clk pc opcode op_a_write_value cols is_real).allHold) :
+--     is_real = 0 ∨ is_real = 1 := by
+--   simp_all [constraints, sub_eq_zero]
 
-/-- `.assertZero E8` -/
-lemma is_real_eq_one_or_imm_c_eq_zero_of_constraints
-    (h : (constraints shard clk pc opcode op_a_write_value cols is_real).allHold) :
-    is_real = 1 ∨ cols.imm_c = 0 := by
-  simp_all [constraints, sub_eq_zero]
+-- /-- `.assertZero E8` -/
+-- lemma is_real_eq_one_or_imm_c_eq_zero_of_constraints
+--     (h : (constraints shard clk pc opcode op_a_write_value cols is_real).allHold) :
+--     is_real = 1 ∨ cols.imm_c = 0 := by
+--   simp_all [constraints, sub_eq_zero]
 
-/-- `.assertZero E14` -/
-lemma op_a_zero_or_op_a_write_values_eq_zero_of_constraints₀
-    (h : (constraints shard clk pc opcode op_a_write_value cols is_real).allHold) :
-    cols.op_a_0 = 0 ∨ op_a_write_value[0] = 0 := by
-  simp_all [constraints, sub_eq_zero]
+-- /-- `.assertZero E14` -/
+-- lemma op_a_zero_or_op_a_write_values_eq_zero_of_constraints₀
+--     (h : (constraints shard clk pc opcode op_a_write_value cols is_real).allHold) :
+--     cols.op_a_0 = 0 ∨ op_a_write_value[0] = 0 := by
+--   simp_all [constraints, sub_eq_zero]
 
-/-- `.assertZero E18` -/
-lemma op_a_zero_or_op_a_write_values_eq_zero_of_constraints₁
-    (h : (constraints shard clk pc opcode op_a_write_value cols is_real).allHold) :
-    cols.op_a_0 = 0 ∨ op_a_write_value[1] = 0 := by
-  simp_all [constraints, sub_eq_zero]
+-- /-- `.assertZero E18` -/
+-- lemma op_a_zero_or_op_a_write_values_eq_zero_of_constraints₁
+--     (h : (constraints shard clk pc opcode op_a_write_value cols is_real).allHold) :
+--     cols.op_a_0 = 0 ∨ op_a_write_value[1] = 0 := by
+--   simp_all [constraints, sub_eq_zero]
 
-lemma op_a_zero_or_op_a_write_values_word_eq_zero_of_constraints
-    (h : (constraints shard clk pc opcode op_a_write_value cols is_real).allHold) :
-    cols.op_a_0 = 0 ∨ Word.toFin32_BB op_a_write_value = 0 := by
-  rw [Word.toFin32_BB]
-  have h0 := op_a_zero_or_op_a_write_values_eq_zero_of_constraints₀ h
-  have h1 := op_a_zero_or_op_a_write_values_eq_zero_of_constraints₁ h
-  rw [or_iff_not_imp_left]
-  intro h
-  simp_all
+-- lemma op_a_zero_or_op_a_write_values_word_eq_zero_of_constraints
+--     (h : (constraints shard clk pc opcode op_a_write_value cols is_real).allHold) :
+--     cols.op_a_0 = 0 ∨ Word.toFin32_BB op_a_write_value = 0 := by
+--   rw [Word.toFin32_BB]
+--   have h0 := op_a_zero_or_op_a_write_values_eq_zero_of_constraints₀ h
+--   have h1 := op_a_zero_or_op_a_write_values_eq_zero_of_constraints₁ h
+--   rw [or_iff_not_imp_left]
+--   intro h
+--   simp_all
 
-/-- `.assertZero E54` NOTE: this one seems strange, should rephrase probably -/
-lemma is_real_sub_imm_c
-    (h : (constraints shard clk pc opcode ap_a_write_value cols is_real).allHold) :
-    is_real - cols.imm_c = 0 ∨ is_real - cols.imm_c = 1 := by
-  simp_all [constraints, sub_eq_zero]
+-- /-- `.assertZero E54` NOTE: this one seems strange, should rephrase probably -/
+-- lemma is_real_sub_imm_c
+--     (h : (constraints shard clk pc opcode ap_a_write_value cols is_real).allHold) :
+--     is_real - cols.imm_c = 0 ∨ is_real - cols.imm_c = 1 := by
+--   simp_all [constraints, sub_eq_zero]
 
-/-- `.assertZero E66` -/
-lemma imm_c_eq_zero_or_prev_value_eq_op_c_of_constraints₀
-    (h : (constraints shard clk pc opcode op_a_write_value cols is_real).allHold) :
-    cols.imm_c = 0 ∨ cols.op_c_memory.prev_value[0] = cols.op_c[0] := by
-  simp_all [constraints, sub_eq_zero]
+-- /-- `.assertZero E66` -/
+-- lemma imm_c_eq_zero_or_prev_value_eq_op_c_of_constraints₀
+--     (h : (constraints shard clk pc opcode op_a_write_value cols is_real).allHold) :
+--     cols.imm_c = 0 ∨ cols.op_c_memory.prev_value[0] = cols.op_c[0] := by
+--   simp_all [constraints, sub_eq_zero]
 
-/-- `.assertZero 70` -/
-lemma imm_c_eq_zero_or_prev_value_eq_op_c_of_constraints₁
-    (h : (constraints shard clk pc opcode op_a_write_value cols is_real).allHold) :
-    cols.imm_c = 0 ∨ cols.op_c_memory.prev_value[1] = cols.op_c[1] := by
-  simp_all [constraints, sub_eq_zero]
+-- /-- `.assertZero 70` -/
+-- lemma imm_c_eq_zero_or_prev_value_eq_op_c_of_constraints₁
+--     (h : (constraints shard clk pc opcode op_a_write_value cols is_real).allHold) :
+--     cols.imm_c = 0 ∨ cols.op_c_memory.prev_value[1] = cols.op_c[1] := by
+--   simp_all [constraints, sub_eq_zero]
 
-lemma imm_c_eq_zero_or_prev_value_eq_op_c
-    (h : (constraints shard clk pc opcode op_a_write_value cols is_real).allHold) :
-    cols.imm_c = 0 ∨ cols.op_c_memory.prev_value = cols.op_c := by
-  have h0 := imm_c_eq_zero_or_prev_value_eq_op_c_of_constraints₀ h
-  have h1 := imm_c_eq_zero_or_prev_value_eq_op_c_of_constraints₁ h
-  rw [Word.ext_cases_iff]
-  aesop
+-- lemma imm_c_eq_zero_or_prev_value_eq_op_c
+--     (h : (constraints shard clk pc opcode op_a_write_value cols is_real).allHold) :
+--     cols.imm_c = 0 ∨ cols.op_c_memory.prev_value = cols.op_c := by
+--   have h0 := imm_c_eq_zero_or_prev_value_eq_op_c_of_constraints₀ h
+--   have h1 := imm_c_eq_zero_or_prev_value_eq_op_c_of_constraints₁ h
+--   rw [Word.ext_cases_iff]
+--   aesop
 
 
-lemma op_b_memory_lt_of_constraints {clk_high clk_low pc opcode : Fin BB}
-    {op_a_write_value : Word (Fin BB)} {cols : ALUTypeReader}
-    (h : (cols.constraints clk_high clk_low pc opcode op_a_write_value 1).allHold) :
-    cols.op_b_memory.prev_value[0] < 65536 ∧ cols.op_b_memory.prev_value[1] < 65536 := by
-  simp [constraints, ByteOpcode.ofNat, Nat.ble, Nat.beq, ByteOpcode.constrain, SP1Constraint.toProp] at h
-  tauto
+-- lemma op_b_memory_lt_of_constraints {clk_high clk_low pc opcode : Fin BB}
+--     {op_a_write_value : Word (Fin BB)} {cols : ALUTypeReader}
+--     (h : (cols.constraints clk_high clk_low pc opcode op_a_write_value 1).allHold) :
+--     cols.op_b_memory.prev_value[0] < 65536 ∧ cols.op_b_memory.prev_value[1] < 65536 := by
+--   simp [constraints, ByteOpcode.ofNat, Nat.ble, Nat.beq, ByteOpcode.constrain, SP1Constraint.toProp] at h
+--   tauto
 
-lemma op_c_memory_lt_of_constraints {clk_high clk_low pc opcode : Fin BB}
-    {op_a_write_value : Word (Fin BB)} {cols : ALUTypeReader}
-    (h : (cols.constraints clk_high clk_low pc opcode op_a_write_value 1).allHold)
-    (himm : cols.imm_c = 0) :
-    cols.op_c_memory.prev_value[0] < 65536 ∧ cols.op_c_memory.prev_value[1] < 65536 := by
-  simp [constraints, ByteOpcode.ofNat, Nat.ble, Nat.beq, ByteOpcode.constrain, SP1Constraint.toProp,
-    sub_eq_zero] at h
-  simp [himm] at h
-  tauto
+-- lemma op_c_memory_lt_of_constraints {clk_high clk_low pc opcode : Fin BB}
+--     {op_a_write_value : Word (Fin BB)} {cols : ALUTypeReader}
+--     (h : (cols.constraints clk_high clk_low pc opcode op_a_write_value 1).allHold)
+--     (himm : cols.imm_c = 0) :
+--     cols.op_c_memory.prev_value[0] < 65536 ∧ cols.op_c_memory.prev_value[1] < 65536 := by
+--   simp [constraints, ByteOpcode.ofNat, Nat.ble, Nat.beq, ByteOpcode.constrain, SP1Constraint.toProp,
+--     sub_eq_zero] at h
+--   simp [himm] at h
+--   tauto
 
-lemma val_op_b_memory_lt_of_constraints {clk_high clk_low pc opcode : Fin BB}
-    {op_a_write_value : Word (Fin BB)} {cols : ALUTypeReader}
-    (h : (cols.constraints clk_high clk_low pc opcode op_a_write_value 1).allHold) :
-    cols.op_b_memory.prev_value[0].val < 65536 ∧ cols.op_b_memory.prev_value[1].val < 65536 := by
-  simp [constraints, ByteOpcode.ofNat, Nat.ble, Nat.beq, ByteOpcode.constrain, SP1Constraint.toProp] at h
-  tauto
+-- lemma val_op_b_memory_lt_of_constraints {clk_high clk_low pc opcode : Fin BB}
+--     {op_a_write_value : Word (Fin BB)} {cols : ALUTypeReader}
+--     (h : (cols.constraints clk_high clk_low pc opcode op_a_write_value 1).allHold) :
+--     cols.op_b_memory.prev_value[0].val < 65536 ∧ cols.op_b_memory.prev_value[1].val < 65536 := by
+--   simp [constraints, ByteOpcode.ofNat, Nat.ble, Nat.beq, ByteOpcode.constrain, SP1Constraint.toProp] at h
+--   tauto
 
-lemma val_op_c_memory_lt_of_constraints {clk_high clk_low pc opcode : Fin BB}
-    {op_a_write_value : Word (Fin BB)} {cols : ALUTypeReader}
-    (h : (cols.constraints clk_high clk_low pc opcode op_a_write_value 1).allHold)
-    (himm : cols.imm_c = 0) :
-    cols.op_c_memory.prev_value[0].val < 65536 ∧ cols.op_c_memory.prev_value[1].val < 65536 := by
-  have := op_c_memory_lt_of_constraints h himm
-  aesop
+-- lemma val_op_c_memory_lt_of_constraints {clk_high clk_low pc opcode : Fin BB}
+--     {op_a_write_value : Word (Fin BB)} {cols : ALUTypeReader}
+--     (h : (cols.constraints clk_high clk_low pc opcode op_a_write_value 1).allHold)
+--     (himm : cols.imm_c = 0) :
+--     cols.op_c_memory.prev_value[0].val < 65536 ∧ cols.op_c_memory.prev_value[1].val < 65536 := by
+--   have := op_c_memory_lt_of_constraints h himm
+--   aesop
 
-end ALUTypeReader
+-- end ALUTypeReader
