SP1Operations/JTypeReader.lean
@@ -1,14 +1,14 @@
-import SP1Foundations
-import SP1Operations.MemoryConsistency
-import LeanRV32IM.RiscvRegs
+-- import SP1Foundations
+-- import SP1Operations.MemoryConsistency
+-- import LeanRV32IM.RiscvRegs
 
-open Sail
-open LeanRV32IM.Functions
+-- open Sail
+-- open LeanRV32IM.Functions
 
---- A Reader that only accesses values of type `T`.
-structure JTypeReader (T : Type) where
-  op_a : T
-  op_a_memory : MemoryAccessInSharedCols
-  op_a_0 : T
-  op_b_imm : Word T
-  op_c_imm : Word T
+-- --- A Reader that only accesses values of type `T`.
+-- structure JTypeReader (T : Type) where
+--   op_a : T
+--   op_a_memory : MemoryAccessInSharedCols
+--   op_a_0 : T
+--   op_b_imm : Word T
+--   op_c_imm : Word T
